Lean4Lean/Experimental/Bridge.lean
@@ -105,8 +105,6 @@ theorem mk_inst_of {a : VExpr} : ∀ {e : VExpr} {k : Nat} {σ : Subst},
   | 0 => rw [VExpr.instVar_zero]; rfl
   | _+1 => rw [VExpr.instVar_upper]; rfl
 
-end SExpr
-
 /-! ## Telescopes
 
 `VIndCtor.type` is `mkPi (C.params ++ C.fields.map (·.type)) (C.canonResult D j)`, and
@@ -128,6 +126,8 @@ theorem mk_mkApp : ∀ {as : List VExpr} {f : VExpr},
 theorem foldr_app_eq_foldl {as : List SExpr} {f : SExpr} :
     as.foldr (fun A acc => acc.app A) f = as.reverse.foldl .app f := by
   simp [List.foldl_reverse]
+
+end SExpr
 
 /-! ## Contexts -/
 
